PokemonLean.lean
@@ -63,3 +63,4 @@ import PokemonLean.TrainerCards
 import PokemonLean.VSTAR
 import PokemonLean.Deck
 import PokemonLean.Tournament
+import PokemonLean.StochasticSemantics
